\documentclass{article}
   \title{Hello World}
   \author {Augusto}
   \usepackage{ctex}
   \usepackage{amssymb}
   \usepackage{amsmath}
\begin{document}
\begin{equation}\label{set}
  D = \{(x_1,y_1),(x_2,y_2),...,(x_m,y_m)\}, x_i \in \mathbb{R}^d, y_i \in \mathbb{R}^l
\end{equation}

\begin{equation}\label{sample}
  (x_k,y_k)
\end{equation}
\begin{equation}\label{output}
  \hat{y}_k = (\hat{y}_1^k, \hat{y}_2^k,...,\hat{y}_l^k)
\end{equation}

\begin{equation}\label{yk}
  \hat{y}_j^k = f(\beta_j - \theta_j)
\end{equation}

\begin{equation}\label{error}
  E_k = \frac{1}{2}\sum\nolimits_{j=1}^{l}( \hat{y}_j^k - y_j^k)^2
\end{equation}

\begin{equation}\label{deltaw}
  \Delta w_{hj} = - \eta \frac{\partial E_k}{\partial w_{hj}}
\end{equation}

\begin{equation}\label{chain}
  \frac{\partial E_k}{\partial w_hj} = \frac{\partial E_k}{\partial \hat{y}_j^k} \cdot \frac{\partial \hat{y}_j^k}{\partial \beta_j} \cdot \frac{\partial \beta_j}{\partial w_{hj}}
\end{equation}

\begin{equation}\label{bh}
  b_h
\end{equation}

\begin{equation}\label{gj}
\begin{split}
  g_j & = - \frac{\partial E_k}{\partial \hat{y}_j^k} \cdot \frac{\partial \hat{y}_j^k}{\partial \beta_j} \\
   & = -(\hat{y}_j^k - y_j^k)f'(\beta_j - \theta_j) \\
   & = \hat{y}_j^k(1- \hat{y}_j^k)(y_j^k - \hat{y}_j^k)
\end{split}
\end{equation}

\begin{equation}\label{whj}
\begin{split}
  \Delta w_{hj} & = - \eta \frac{\partial E_k}{\partial w_{hj}} \\
   & = \eta g_j b_h
\end{split}
\end{equation}

\begin{equation}\label{sigmoidpartial}
\begin{split}
  f(x) & = \frac{1}{1 + e ^{-x}} \\
  f(x)' & = f(x)(1-f(x))
\end{split}
\end{equation}

\begin{equation}\label{ykj}
  \hat{y}_j^k = f(\beta _j - \theta _j)
\end{equation}

\begin{equation}\label{thetaj}
\begin{split}
  \Delta \theta _j & = - \eta g_j \\
  \Delta v_{ih} & = \eta e_hx_i \\
  \Delta \gamma _h & = - \eta e_h
\end{split}
\end{equation}

\begin{equation}\label{eh}
  \begin{split}
     e_h & = - \frac{\partial E_k}{\partial b_h} \cdot \frac{\partial b_h}{\partial \alpha _h} \\
       & =  - \sum\nolimits_{j=1}^{l} \frac{\partial E_k}{\partial \beta _j} \cdot \frac{\partial \beta _j}{\partial b_h} f'(\alpha _h - \gamma _h)  \\
       & = \sum\nolimits_{j=1}^{l}w_{hj}g_jf'(\alpha _h - \gamma _h) \\
       &  = b_h(1 - b_h) \sum\nolimits_{j-1}^{l}w_{hj}g_j
  \end{split}
\end{equation}

\begin{equation}\label{E }
  E = \lambda \frac{1}{m}\sum\nolimits_{k=1}^{m}E_k + (1 - \lambda)\sum\nolimits_{i}w_i^2
\end{equation}

\begin{equation}\label{rbff}
  \rho(x,c_i) = e^{-\beta _i\left\|x-c_i\right\|^2}
\end{equation}
\begin{equation}\label{rbfl}
  \varphi(x) = \sum\nolimits_{i=1}^{q}w_i \rho (x,c_i)
\end{equation}

\begin{equation}\label{relu}
  f(x) = \left\{ \begin{array}{cc}
                   0, & \text{ if $x < 0$, }\\
                   x, & \text{  otherwise,}
                 \end{array}\right.
\end{equation}




\end{document}