\documentclass{article}
   \title{Hello World}
   \author {Augusto}
   \usepackage{ctex}
   \usepackage{amssymb}
   \usepackage{amsmath}
\begin{document}
\begin{equation}\label{wx}
  y = wx
\end{equation}

\begin{equation}\label{1}
  w^T \cdot x +b = 0
\end{equation}

\begin{equation}\label{r}
  r = \frac{\left|w^T \cdot x + b\right|}{||w||}
\end{equation}

\begin{equation}\label{gamma}
  \gamma  = \frac{2}{||w||}
\end{equation}

\begin{equation}\label{fx}
  \left\{ \begin{array}{cc}
            w^Tx_i + b \geq +1, & y_i = +1 \\
            w^Tx_i + b \leq -1, & y_i = -1
          \end{array}\right.
\end{equation}

\begin{equation}\label{tar}
  \mathop{\arg\min}_{(w,b)} \frac{2}{||w||}
\end{equation}

\begin{equation}\label{y}
  y_i(w^Tx_i + b) \geq 1, i = 1,2,...,m
\end{equation}

\begin{equation}\label{e}
  \mathop{\arg\min}_{(w,b)} \frac{1}{2}{||w||}^2
\end{equation}

\begin{equation}\label{e2}
  y_i(w^Tx_i + b) \geq 1, i = i,2,...,m
\end{equation}

\begin{equation}\label{dual}
  L(w,b,\alpha) = \frac{1}{2} {||w||}^2 + \sum\nolimits_{i=1}^{m}\alpha_i(1 - y_i(w^Tx_i+b))
\end{equation}

\begin{equation}\label{partialderivative}
 \begin{split}
     & w = \sum\nolimits_{i=1}^{m}\alpha_iy_ix_i \\
      & 0 = \sum\nolimits_{i=1}^{m}\alpha_iy_i
 \end{split}
\end{equation}

\begin{equation}\label{alpha}
\begin{split}
     \mathop{\max}_{\alpha} & \sum\nolimits_{i = 1}^{m} \alpha_i - \frac{1}{2} \sum\nolimits_{i=1}^{m}\sum\nolimits_{j=1}^{m} \alpha_i \alpha_j y_i y_jx_i^Tx_j \\
     s.t. & \sum\nolimits_{i=1}^{m}\alpha_iy_i = 0, \alpha_i \geq 0, i = 1,2,...,m
\end{split}
\end{equation}

\begin{equation}\label{model}
\begin{split}
   f(x) & = w^Tx + b \\
     & = \sum\nolimits_{i=1}^{m}\alpha_iy_ix_i^Tx+b
\end{split}
\end{equation}


\begin{equation}\label{constraints}
  \left\{ \begin{aligned}
            & \alpha_i \geq 0; \\
            & y_if(x_i) -1 \geq 0; \\
            & \alpha_i(y_if(x_i) -1) = 0
          \end{aligned}\right.
\end{equation}

\begin{equation}\label{tt}
\begin{aligned}
   \mathop{\arg\min}_{(w,b)}  &  \text{ }\frac{1}{2}{||w||}^2 \\
  s.t. & \text{ }  y_i(w^T\phi(x_i) + b) \geq 1, i = 1,2,...,m
\end{aligned}
\end{equation}

\begin{equation}\label{ttd}
\begin{aligned}
  \mathop{\max}_{\alpha} & \space \sum\nolimits_{i = 1}^{m} \alpha_i - \frac{1}{2} \sum\nolimits_{i=1}^{m}\sum\nolimits_{j=1}^{m} \alpha_i \alpha_j y_i y_j{\phi(x_i)}^T\phi(x_j) \\
     s.t. &\space \sum\nolimits_{i=1}^{m}\alpha_iy_i = 0, \alpha_i \geq 0, i = 1,2,...,m
\end{aligned}
\end{equation}

\begin{equation}\label{predd}
  f(x) = w^T\phi(x) + b = \sum\nolimits_{i=1}^{m}\alpha_iy_i{\phi(x_i)}^T\phi(x) + b
\end{equation}

\begin{equation}\label{kernel}
  \kappa(x_i,x_j) = \phi(x_i)^T\phi(x_j)
\end{equation}

\begin{equation}\label{p1}
  \gamma_1\kappa_1 + \gamma_2\kappa_2
\end{equation}
\begin{equation}\label{p2}
  \kappa_1 \otimes \kappa_2(x,z) = \kappa_1(x,z)\kappa_2(x,z)
\end{equation}

\begin{equation}\label{p3}
  \kappa(x,z) = g(x)\kappa_1(x,z)g(z)
\end{equation}

\end{document}